3.4/LanguageModuleDef.v
@@ -18,28 +18,37 @@ Require Export TauModuleDef.
 Require Export PathModuleDef.
 Require Export PhiModuleDef.
 Require Export TermModuleDef.
+Require Export ContextFunDef.
+
+(* Modules:
+   kappa - K
+   phi   - P
+   Path  - Path
+   Tau   - T
+   Term  - TM
+   TVar - TV.
+   TVars - TVS.
+   EVar - EV.
+   EVars - EVS.
+*)
 
 Module LanguageModule.
-  Module T   := TauModule.
-  Include T.Types.
-  Definition TVar := T.TV.t.
-  (* Paths come from terms. *)
-  Module Pth := PathModule.   
-
-  Export TermModule.
   Module TM := TermModule.
-  (* I'd have to functorize this to show the dependencies to TM.EV and Path and so on. *)
   Include TM.Types.
-
-  Definition EVar := TM.EVar.
-
-  Module EVP := EVarPathModule.
-
-  Module D := ContextFun T.TV T.K.
+(*
+  Print Module K.
+  Print Module P.
+  Print Module Path.
+  Print Module T.
+  Print Module TM.
+  Print Module TV.
+  Print Module TVS.
+  Print Module EV.
+  Print Module EVS.
+*)
+  Module D := ContextFun TV K.
   (* Now what happens here if I use D.K/D.T vs TV.T T.K ? *)
   Definition Delta    := D.Context.
-  Module TVSM         := D.KSet.
-
 
   (* Can I just drop these and get rid of some unfolding? Seems likely. *)
   Notation "x '~_d' a" := (D.ctxt x a D.dot)
@@ -47,16 +56,8 @@ Module LanguageModule.
   Notation "E '&_d' F" := (D.concat E F) 
                            (at level 28, left associativity).
 
-  Module U := ContextFun EVarPathModule T.
-  Definition Upsilon  := U.Context.
-
-  Module H := ContextFun TM.EV TM.
-  Definition Heap     := H.Context.
-
-  Module G := ContextFun TM.EV T.
+  Module G := ContextFun EV T.
   Definition Gamma    := G.Context.
-  Module EVSM         := G.KSet.
-
 
   Notation "x '~_g' a" := (G.ctxt x a G.dot)
                            (at level 27, left associativity).
@@ -65,32 +66,39 @@ Module LanguageModule.
 
 
 
-  Notation "\{}_t" := (TVSM.empty).
-  Notation "\{ x }_t" := (TVSM.singleton x).
-  Notation "E \u_t F" := (TVSM.union E F)
+
+  Module U := ContextFun EVarPathModule T.
+  Definition Upsilon  := U.Context.
+
+  Module H := ContextFun EV TM.
+  Definition Heap     := H.Context.
+
+
+  Notation "\{}_t" := (TVS.empty).
+  Notation "\{ x }_t" := (TVS.singleton x).
+  Notation "E \u_t F" := (TVS.union E F)
                            (at level 37, right associativity).
-  Notation "E \n_t F" := (TVSM.inter E F)
+  Notation "E \n_t F" := (TVS.inter E F)
                            (at level 36, right associativity).
-  Notation "E \-_t F" := (TVSM.remove E F)
+  Notation "E \-_t F" := (TVS.remove E F)
                            (at level 35).
-  Notation "x \in_t E" := ((TVSM.mem x E) = true) (at level 39).
-  Notation "x \notin_t E" := ((TVSM.mem x E) = false) (at level 39).
-  Notation "E \c_t F" := (TVSM.subset E F)
+  Notation "x \in_t E" := ((TVS.mem x E) = true) (at level 39).
+  Notation "x \notin_t E" := ((TVS.mem x E) = false) (at level 39).
+  Notation "E \c_t F" := (TVS.subset E F)
                            (at level 38).
 
-  Notation "\{}_e" := (EVSM.empty).
-  Notation "\{ x }_e" := (EVSM.singleton x).
-  Notation "E \u_e F" := (EVSM.union E F)
+  Notation "\{}_e" := (EVS.empty).
+  Notation "\{ x }_e" := (EVS.singleton x).
+  Notation "E \u_e F" := (EVS.union E F)
                            (at level 37, right associativity).
-  Notation "E \n_e F" := (EVSM.inter E F)
+  Notation "E \n_e F" := (EVS.inter E F)
                            (at level 36, right associativity).
-  Notation "E \-_e F" := (EVSM.remove E F)
+  Notation "E \-_e F" := (EVS.remove E F)
                            (at level 35).
-  Notation "x \in_e E" := ((EVSM.mem x E) = true) (at level 39).
-  Notation "x \notin_e E" := ((EVSM.mem x E) = false) (at level 39).
-  Notation "E \c_e F" := (EVSM.subset E F)
+  Notation "x \in_e E" := ((EVS.mem x E) = true) (at level 39).
+  Notation "x \notin_e E" := ((EVS.mem x E) = false) (at level 39).
+  Notation "E \c_e F" := (EVS.subset E F)
                            (at level 38).
 
 End LanguageModule.
-
 Export LanguageModule.
